Fixed inconsistency between proofs and paper

isabelle/List_Spec.thy
@@ -2,26 +2,25 @@ theory List_Spec
   imports Insert_Spec
 begin
 
-fun succ_rel :: "'oid list \<Rightarrow> ('oid \<times> 'oid) set" where
+fun succ_rel :: "'oid list \<Rightarrow> ('oid \<times> 'oid option) set" where
   "succ_rel [] = {}" |
-  "succ_rel [head] = {}" |
-  "succ_rel (head#x#xs) = {(head, x)} \<union> succ_rel (x#xs)"
+  "succ_rel [head] = {(head, None)}" |
+  "succ_rel (head#x#xs) = {(head, Some x)} \<union> succ_rel (x#xs)"
 
-fun insert_spec_alt :: "('oid \<times> 'oid) set \<Rightarrow> ('oid \<times> 'oid) \<Rightarrow> ('oid \<times> 'oid) set" where
-  "insert_spec_alt list_rel (oid, ref) = (
-      {(p, n) \<in> list_rel. p \<noteq> ref} \<union> {(ref, oid)} \<union>
-      {(i, n). i = oid \<and> (ref, n) \<in> list_rel})"
+fun insert_alt :: "('oid \<times> 'oid option) set \<Rightarrow> ('oid \<times> 'oid) \<Rightarrow> ('oid \<times> 'oid option) set" where
+  "insert_alt list_rel (oid, ref) = (
+      if \<exists>n. (ref, n) \<in> list_rel
+      then {(p, n) \<in> list_rel. p \<noteq> ref} \<union> {(ref, Some oid)} \<union>
+           {(i, n). i = oid \<and> (ref, n) \<in> list_rel}
+      else list_rel)"
 
 lemma succ_rel_set_fst:
-  shows "fst ` (succ_rel xs) = set (butlast xs)"
-by (induction xs rule: succ_rel.induct, auto)
-
-lemma succ_rel_set_snd:
-  shows "snd ` (succ_rel xs) = set (tl xs)"
+  shows "fst ` (succ_rel xs) = set xs"
 by (induction xs rule: succ_rel.induct, auto)
 
 lemma succ_rel_functional:
-  assumes "{(a, b1), (a, b2)} \<subseteq> succ_rel xs"
+  assumes "(a, b1) \<in> succ_rel xs"
+    and "(a, b2) \<in> succ_rel xs"
     and "distinct xs"
   shows "b1 = b2"
 using assms proof(induction xs rule: succ_rel.induct)
@@ -38,7 +37,7 @@ next
     hence "a \<notin> set (x#xs)"
       using 3 by blast
     hence "a \<notin> fst ` (succ_rel (x#xs))"
-      using succ_rel_set_fst in_set_butlastD by metis
+      using succ_rel_set_fst by metis
     then show "b1 = b2"
       using 3 image_iff by fastforce
   next
@@ -48,85 +47,228 @@ next
     moreover have "distinct (x#xs)"
       using 3 by auto
     ultimately show "b1 = b2"
-      using "3.IH" by linarith
+      using "3.IH" by auto
   qed
 qed
 
 lemma succ_rel_rem_head:
-  assumes "distinct (x#y#xs)"
-  shows "{(p, n) \<in> succ_rel (x#y#xs). p \<noteq> x} = succ_rel (y#xs)"
+  assumes "distinct (x # xs)"
+  shows "{(p, n) \<in> succ_rel (x # xs). p \<noteq> x} = succ_rel xs"
 proof -
-  have head_notin: "x \<notin> fst ` succ_rel (y#xs)"
-    using assms succ_rel_set_fst by (metis distinct_set_notin in_set_butlastD)
-  moreover have "succ_rel (x#y#xs) = {(x, y)} \<union> succ_rel (y#xs)"
-    by simp
-  moreover from this have "\<And>n. (x, n) \<in> succ_rel (x#y#xs) \<Longrightarrow> n = y"
+  have head_notin: "x \<notin> fst ` succ_rel xs"
+    using assms succ_rel_set_fst by (metis distinct_set_notin)
+  moreover obtain y where "(x, y) \<in> succ_rel (x # xs)"
+    by (cases xs, auto)
+  moreover have "succ_rel (x # xs) = {(x, y)} \<union> succ_rel xs"
+    using calculation head_notin image_iff by (cases xs, fastforce+)
+  moreover from this have "\<And>n. (x, n) \<in> succ_rel (x # xs) \<Longrightarrow> n = y"
     by (metis Pair_inject fst_conv head_notin image_eqI insertE insert_is_Un)
-  hence "{(p, n) \<in> succ_rel (x#y#xs). p \<noteq> x} = succ_rel (x#y#xs) - {(x, y)}"
+  hence "{(p, n) \<in> succ_rel (x # xs). p \<noteq> x} = succ_rel (x # xs) - {(x, y)}"
     by blast
-  moreover have "succ_rel (x#y#xs) - {(x, y)} = succ_rel (y#xs)"
-    using head_notin image_iff by fastforce
-  ultimately show "{(p, n) \<in> succ_rel (x#y#xs). p \<noteq> x} = succ_rel (y#xs)"
+  moreover have "succ_rel (x # xs) - {(x, y)} = succ_rel xs"
+    using image_iff calculation by fastforce
+  ultimately show "{(p, n) \<in> succ_rel (x # xs). p \<noteq> x} = succ_rel xs"
     by simp
 qed
 
+lemma succ_rel_swap_head:
+  assumes "distinct (ref # list)"
+    and "(ref, n) \<in> succ_rel (ref # list)"
+  shows "succ_rel (oid # list) = {(oid, n)} \<union> succ_rel list"
+proof(cases list)
+  case Nil
+  then show ?thesis using assms by auto
+next
+  case (Cons a list)
+  moreover from this have "n = Some a"
+    by (metis Un_iff assms singletonI succ_rel.simps(3) succ_rel_functional)
+  ultimately show ?thesis by simp
+qed
 
-lemma insert_spec_succ_rel:
-  assumes "after = insert_spec before (oid, if ref = head then None else Some ref)"
-    and "distinct (head # oid # before)"
-  shows "succ_rel (head # after) = insert_spec_alt (succ_rel (head # before)) (oid, ref)"
-proof(cases "ref = head")
-  case ref_head: True
-  hence "after = oid # before"
-    using assms by simp
-  then show ?thesis
-  proof(cases before)
-    case before_empty: Nil
-    moreover from this have "succ_rel (head # before) = {}"
-      by simp
-    moreover from this have "succ_rel (head # after) = {(head, oid)}"
-      using \<open>after = oid # before\<close> before_empty by auto
-    ultimately show ?thesis 
-      using ref_head by auto
-  next
-    case (Cons a list)
-    moreover from this have head_in_rel: "(head, a) \<in> succ_rel (head # before)"
-      by (cases list, auto)
-    moreover have "distinct (head#a#list)"
-      using assms(2) calculation by auto
-    hence "{(p, n) \<in> succ_rel (head#a#list). p \<noteq> head} = succ_rel (a#list)"
-      using succ_rel_rem_head by fastforce
-    hence "{(p, n) \<in> succ_rel (head#before). p \<noteq> ref} = succ_rel before"
-      using local.Cons ref_head by auto
-    moreover have "{(i, n). i = oid \<and> (ref, n) \<in> succ_rel (head # before)} = {(oid, a)}"
-    proof -
-      have "\<And>n. (head, n) \<in> succ_rel (head # before) \<Longrightarrow> n = a"
-        using calculation succ_rel_rem_head ref_head by fastforce
-      hence "{(i, n) \<in> succ_rel (head # before). i = head} \<subseteq> {(head, a)}"
-        by blast
-      moreover have "{(head, a)} \<subseteq> {(i, n) \<in> succ_rel (head # before). i = head}"
-        by (simp add: head_in_rel)
-      ultimately show ?thesis
-        using ref_head by blast
-    qed
-    moreover have "succ_rel before = succ_rel (tl after)"
-      by (simp add: \<open>after = oid # before\<close>)
-    moreover have "insert_spec_alt (succ_rel (head # before)) (oid, ref) =
-                     {(p, n) \<in> succ_rel (head # before). p \<noteq> ref} \<union> {(ref, oid)} \<union>
-                     {(i, n). i = oid \<and> (ref, n) \<in> succ_rel (head # before)}"
-      by simp
-    ultimately have "insert_spec_alt (succ_rel (head # before)) (oid, ref) =
-             succ_rel (a#list) \<union> {(ref, oid)} \<union> {(oid, a)}"
-      by simp
-    moreover have "succ_rel (head # after) = {(head, oid), (oid, a)} \<union> succ_rel before"
-      using \<open>after = oid # before\<close> local.Cons by auto
-    ultimately show ?thesis
-      using local.Cons ref_head by auto
+lemma succ_rel_insert_alt:
+  assumes "a \<noteq> ref"
+    and "distinct (oid # a # b # list)"
+  shows "insert_alt (succ_rel (a # b # list)) (oid, ref) =
+         {(a, Some b)} \<union> insert_alt (succ_rel (b # list)) (oid, ref)"
+proof(cases "\<exists>n. (ref, n) \<in> succ_rel (a # b # list)")
+  case True
+  hence "insert_alt (succ_rel (a # b # list)) (oid, ref) =
+           {(p, n) \<in> succ_rel (a # b # list). p \<noteq> ref} \<union> {(ref, Some oid)} \<union>
+           {(i, n). i = oid \<and> (ref, n) \<in> succ_rel (a # b # list)}"
+    by simp
+  moreover have "{(p, n) \<in> succ_rel (a # b # list). p \<noteq> ref} =
+                 {(a, Some b)} \<union> {(p, n) \<in> succ_rel (b # list). p \<noteq> ref}"
+    using assms(1) by auto
+  moreover have "insert_alt (succ_rel (b # list)) (oid, ref) =
+           {(p, n) \<in> succ_rel (b # list). p \<noteq> ref} \<union> {(ref, Some oid)} \<union>
+           {(i, n). i = oid \<and> (ref, n) \<in> succ_rel (b # list)}"
+  proof -
+    have "\<exists>n. (ref, n) \<in> succ_rel (b # list)"
+      using assms(1) True by auto
+    thus ?thesis by simp
   qed
+  moreover have "{(i, n). i = oid \<and> (ref, n) \<in> succ_rel (a # b # list)} =
+                 {(i, n). i = oid \<and> (ref, n) \<in> succ_rel (b # list)}"
+    using assms(1) by auto
+  ultimately show ?thesis by simp
 next
   case False
-  then show ?thesis sorry
+  then show ?thesis by auto
 qed
-  
+
+lemma succ_rel_insert_head:
+  assumes "distinct (ref # list)"
+  shows "succ_rel (insert_spec (ref # list) (oid, Some ref)) =
+         insert_alt (succ_rel (ref # list)) (oid, ref)"
+proof -
+  obtain n where ref_in_rel: "(ref, n) \<in> succ_rel (ref # list)"
+    by (cases list, auto)
+  moreover from this have "{(p, n) \<in> succ_rel (ref # list). p \<noteq> ref} = succ_rel list"
+    using assms succ_rel_rem_head by (metis (mono_tags, lifting))
+  moreover have "{(i, n). i = oid \<and> (ref, n) \<in> succ_rel (ref # list)} = {(oid, n)}"
+  proof -
+    have "\<And>nx. (ref, nx) \<in> succ_rel (ref # list) \<Longrightarrow> nx = n"
+      using assms by (simp add: succ_rel_functional ref_in_rel)
+    hence "{(i, n) \<in> succ_rel (ref # list). i = ref} \<subseteq> {(ref, n)}"
+      by blast
+    moreover have "{(ref, n)} \<subseteq> {(i, n) \<in> succ_rel (ref # list). i = ref}"
+      by (simp add: ref_in_rel)
+    ultimately show ?thesis by blast
+  qed
+  moreover have "insert_alt (succ_rel (ref # list)) (oid, ref) =
+                   {(p, n) \<in> succ_rel (ref # list). p \<noteq> ref} \<union> {(ref, Some oid)} \<union>
+                   {(i, n). i = oid \<and> (ref, n) \<in> succ_rel (ref # list)}"
+  proof -
+    have "\<exists>n. (ref, n) \<in> succ_rel (ref # list)"
+      using ref_in_rel by blast
+    thus ?thesis by simp
+  qed
+  ultimately have "insert_alt (succ_rel (ref # list)) (oid, ref) =
+                   succ_rel list \<union> {(ref, Some oid)} \<union> {(oid, n)}"
+    by simp
+  moreover have "succ_rel (oid # list) = {(oid, n)} \<union> succ_rel list"
+    using assms ref_in_rel succ_rel_swap_head by metis
+  hence "succ_rel (ref # oid # list) = {(ref, Some oid), (oid, n)} \<union> succ_rel list"
+    by auto
+  ultimately show "succ_rel (insert_spec (ref # list) (oid, Some ref)) =
+                   insert_alt (succ_rel (ref # list)) (oid, ref)"
+    by auto
+qed
+
+lemma succ_rel_insert_later:
+  assumes "succ_rel (insert_spec (b # list) (oid, Some ref)) =
+           insert_alt (succ_rel (b # list)) (oid, ref)"
+    and "a \<noteq> ref"
+    and "distinct (a # b # list)"
+  shows "succ_rel (insert_spec (a # b # list) (oid, Some ref)) =
+         insert_alt (succ_rel (a # b # list)) (oid, ref)"
+proof -
+  have "succ_rel (a # b # list) = {(a, Some b)} \<union> succ_rel (b # list)"
+    by simp
+  moreover have "insert_spec (a # b # list) (oid, Some ref) =
+                 a # (insert_spec (b # list) (oid, Some ref))"
+    using assms(2) by simp
+  hence "succ_rel (insert_spec (a # b # list) (oid, Some ref)) =
+         {(a, Some b)} \<union> succ_rel (insert_spec (b # list) (oid, Some ref))"
+    by auto
+  hence "succ_rel (insert_spec (a # b # list) (oid, Some ref)) =
+         {(a, Some b)} \<union> insert_alt (succ_rel (b # list)) (oid, ref)"
+    using assms(1) by auto
+  moreover have "insert_alt (succ_rel (a # b # list)) (oid, ref) =
+                 {(a, Some b)} \<union> insert_alt (succ_rel (b # list)) (oid, ref)"
+    using succ_rel_insert_alt assms(2) by auto
+  ultimately show ?thesis by blast
+qed
+
+lemma succ_rel_insert_Some:
+  assumes "distinct list"
+  shows "succ_rel (insert_spec list (oid, Some ref)) = insert_alt (succ_rel list) (oid, ref)"
+using assms proof(induction list)
+  case Nil
+  then show "succ_rel (insert_spec [] (oid, Some ref)) = insert_alt (succ_rel []) (oid, ref)"
+    by simp
+next
+  case (Cons a list)
+  hence "distinct (a # list)"
+    by simp
+  then show "succ_rel (insert_spec (a # list) (oid, Some ref)) =
+             insert_alt (succ_rel (a # list)) (oid, ref)"
+  proof(cases "a = ref")
+    case True
+    then show ?thesis
+      using succ_rel_insert_head \<open>distinct (a # list)\<close> by metis
+  next
+    case False
+    hence "a \<noteq> ref" by simp
+    moreover have "succ_rel (insert_spec list (oid, Some ref)) =
+                   insert_alt (succ_rel list) (oid, ref)"
+      using Cons.IH Cons.prems by auto
+    ultimately show "succ_rel (insert_spec (a # list) (oid, Some ref)) =
+                     insert_alt (succ_rel (a # list)) (oid, ref)"
+      by (cases list, force, metis Cons.prems succ_rel_insert_later)
+  qed
+qed
+
+definition interp_alt :: "'oid \<Rightarrow> ('oid \<times> 'oid option) list \<Rightarrow> ('oid \<times> 'oid option) set" where
+  "interp_alt head ops \<equiv> foldl insert_alt {(head, None)}
+     (map (\<lambda>x. case x of
+            (oid, None)     \<Rightarrow> (oid, head) |
+            (oid, Some ref) \<Rightarrow> (oid, ref)) 
+      ops)"
+
+theorem insert_alt_equivalent:
+  assumes "list_spec ops"
+    and "head \<notin> fst ` set ops"
+    and "\<And>r. Some r \<in> snd ` set ops \<Longrightarrow> r \<noteq> head"
+  shows "succ_rel (head # interp_list ops) = interp_alt head ops"
+using assms proof(induction ops rule: List.rev_induct)
+  case Nil
+  then show "succ_rel (head # interp_list []) = interp_alt head []"
+    by (simp add: interp_list_def interp_alt_def)
+next
+  case (snoc x xs)
+  have IH: "succ_rel (head # interp_list xs) = interp_alt head xs"
+    using snoc by auto
+  have distinct_list: "distinct (head # interp_list xs)"
+  proof -
+    have "distinct (interp_list xs)"
+      using interp_list_distinct snoc.prems(1) by blast
+    moreover have "set (interp_list xs) \<subseteq> fst ` set xs"
+      using interp_list_subset snoc.prems(1) by fastforce
+    ultimately show "distinct (head # interp_list xs)"
+      using snoc.prems(2) by auto
+  qed
+  obtain oid r where x_pair: "x = (oid, r)" by force
+  then show "succ_rel (head # interp_list (xs @ [x])) = interp_alt head (xs @ [x])"
+  proof(cases r)
+    case None
+    have "interp_alt head (xs @ [x]) = insert_alt (interp_alt head xs) (oid, head)"
+      by (simp add: interp_alt_def None x_pair)
+    moreover have "... = insert_alt (succ_rel (head # interp_list xs)) (oid, head)"
+      by (simp add: IH)
+    moreover have "... = succ_rel (insert_spec (head # interp_list xs) (oid, Some head))"
+      using distinct_list succ_rel_insert_Some by metis
+    moreover have "... = succ_rel (head # (insert_spec (interp_list xs) (oid, None)))"
+      by auto
+    moreover have "... = succ_rel (head # (interp_list (xs @ [x])))"
+      by (simp add: interp_list_tail_unfold None x_pair)
+    ultimately show ?thesis by simp
+  next
+    case (Some ref)
+    have "ref \<noteq> head"
+      by (simp add: Some snoc.prems(3) x_pair)
+    have "interp_alt head (xs @ [x]) = insert_alt (interp_alt head xs) (oid, ref)"
+      by (simp add: interp_alt_def Some x_pair)
+    moreover have "... = insert_alt (succ_rel (head # interp_list xs)) (oid, ref)"
+      by (simp add: IH)
+    moreover have "... = succ_rel (insert_spec (head # interp_list xs) (oid, Some ref))"
+      using distinct_list succ_rel_insert_Some by metis
+    moreover have "... = succ_rel (head # (insert_spec (interp_list xs) (oid, Some ref)))"
+      using \<open>ref \<noteq> head\<close> by auto
+    moreover have "... = succ_rel (head # (interp_list (xs @ [x])))"
+      by (simp add: interp_list_tail_unfold Some x_pair)
+    ultimately show ?thesis by simp
+  qed
+qed
 
 end
