isabelle/Insert_Spec.thy
@@ -150,60 +150,37 @@ next
   qed
 qed
 
+lemma interp_list_subset [simp]:
+  assumes "list_spec op_list"
+  shows "set (interp_list op_list) \<subseteq> set (map fst op_list)"
+using assms proof(induction op_list rule: List.rev_induct)
+  case Nil
+  then show "set (interp_list []) \<subseteq> set (map fst [])"
+    by (simp add: interp_list_def)
+next
+  case (snoc x xs)
+  hence IH: "set (interp_list xs) \<subseteq> set (map fst xs)"
+    by blast
+  obtain oid ref where x_pair: "x = (oid, ref)"
+    by fastforce
+  hence spec: "interp_list (xs @ [x]) = insert_spec (interp_list xs) (oid, ref)"
+    by (simp add: interp_list_def)
+  then show "set (interp_list (xs @ [x])) \<subseteq> set (map fst (xs @ [x]))"
+  proof(cases ref)
+    case None
+    then show "set (interp_list (xs @ [x])) \<subseteq> set (map fst (xs @ [x]))"
+      using IH spec x_pair by auto
+  next
+    case (Some a)
+    then show "set (interp_list (xs @ [x])) \<subseteq> set (map fst (xs @ [x]))"
+      using IH spec x_pair by (cases "a \<in> set (interp_list xs)", auto)
+  qed
+qed
+
 lemma list_oid_subset [simp]:
   assumes "list_spec op_list"
   shows "set (list_spec.ins_list op_list) \<subseteq> set (map fst op_list)"
-using assms proof(induction op_list rule: List.rev_induct)
-  show "set (list_spec.ins_list []) \<subseteq> set (map fst [])"
-    by(auto simp add: list_spec.ins_list_def[OF list_spec_NilI] interp_list_def)
-next
-  fix x and xs :: "('a \<times> 'a option) list"
-  assume "list_spec xs \<Longrightarrow> set (list_spec.ins_list xs) \<subseteq> set (map fst xs)"
-    and S: "list_spec (xs@[x])"
-  hence IH: "set (list_spec.ins_list xs) \<subseteq> set (map fst xs)"
-    by blast
-  obtain id ref where P: "x = (id, ref)"
-    by fastforce
-  show "set (list_spec.ins_list (xs@[x])) \<subseteq> set (map fst (xs@[x]))"
-  proof -
-    {
-      fix e
-      assume 1: "e \<in> set (list_spec.ins_list (xs @ [(id, ref)]))"
-        and 2: "e \<notin> fst ` set xs"
-      have 3: "list_spec (xs @ [(id, ref)])"
-        using S P by auto
-      obtain f where F: "foldl insert_spec [] xs = f"
-        by fastforce
-      hence 4: "e \<in> set (insert_spec f (id, ref))"
-        using 1 2 3 by(clarsimp simp add: list_spec.ins_list_def interp_list_def)
-      have "e = id"
-      proof(cases ref)
-        assume "ref = None"
-        thus "e = id"
-          using 2 4 F IH S by(metis contra_subsetD  image_set insert_spec.simps(1)
-              interp_list_def list_spec.ins_list_def list_spec_rm_last set_ConsD)
-      next
-        fix a
-        assume "ref = Some a"
-        show "e = id"
-        proof(cases "a \<in> set f")
-          assume "a \<in> set f"
-          show "e = id"
-            using 2 3 4 IH F by(metis \<open>a \<in> set f\<close> \<open>ref = Some a\<close> contra_subsetD image_set
-                insert_spec.simps(1) insert_spec_none insert_spec_set interp_list_def
-                list_spec.ins_list_def list_spec_rm_last set_ConsD)
-        next
-          assume "a \<notin> set f"
-          show "e = id"
-            using 2 3 4 IH F by(metis \<open>a \<notin> set f\<close> \<open>ref = Some a\<close> contra_subsetD image_set
-                insert_spec_nonex interp_list_def list_spec.ins_list_def list_spec_rm_last)
-        qed
-      qed 
-    }
-    thus "set (list_spec.ins_list (xs@[x])) \<subseteq> set (map fst (xs@[x]))"
-      by(clarsimp simp add: P)
-  qed
-qed
+using assms interp_list_subset list_spec.ins_list_def by fastforce
 
 lemma inserted_item_ident:
   assumes "a \<in> set (insert_spec xs (e, i))"
@@ -271,18 +248,30 @@ next
   qed
 qed
 
+lemma interp_list_distinct:
+  assumes "list_spec op_list"
+  shows "distinct (interp_list op_list)"
+using assms proof(induction op_list rule: rev_induct)
+  case Nil
+  then show "distinct (interp_list [])"
+    by (simp add: interp_list_def)
+next
+  case (snoc x xs)
+  hence IH: "distinct (interp_list xs)" by blast
+  obtain oid ref where x_pair: "x = (oid, ref)" by force
+  hence "\<forall>x\<in>set (list_spec.ins_list xs). x < oid"
+    using last_op_greatest list_oid_subset snoc.prems by blast
+  hence "distinct (insert_spec (interp_list xs) (oid, ref))"
+    using IH insert_spec_distinct
+    by (metis insert_spec_nonex list_spec.ins_list_def list_spec_rm_last snoc.prems)
+  then show "distinct (interp_list (xs @ [x]))"
+    by (simp add: x_pair interp_list_tail_unfold)
+qed
+
 lemma list_distinct:
   assumes "list_spec op_list"
   shows "distinct (list_spec.ins_list op_list)"
-  using assms apply (induct op_list rule: rev_induct)
-  apply(simp add: list_spec.ins_list_def interp_list_def)
-  apply(frule list_spec_rm_last, clarsimp)
-  apply(subgoal_tac "\<forall>x\<in>set (list_spec.ins_list xs). x < a") prefer 2
-  using last_op_greatest list_oid_subset apply blast
-  apply(subgoal_tac "distinct (insert_spec (list_spec.ins_list xs) (a, b))") prefer 2
-  apply(metis insert_spec.simps(2) insert_spec_distinct last_in_set)
-  apply(simp add: list_spec.ins_list_def interp_list_def)
-  done
+using assms by (simp add: interp_list_distinct list_spec.ins_list_def)
 
 lemma suffix_eq_distinct_list:
   assumes "ys@suf1 = xs"
